Hacl.Impl.QTesla.fst almost free of assumptions
shift_arithmetic_left assumptions still exist as that work is in progress with Santiago.

Remaining assumptions are all about disjointness or modifies which are provable, but require very expensive lemmas to be enabled.

qtesla/code/Hacl.Impl.QTesla.fst
@@ -1967,12 +1967,12 @@ val test_z:
     z : poly
   -> Stack (r:I32.t{r == 0l \/ r == 1l})
     (requires fun h -> live h z)
-    (ensures fun h0 _ h1 -> h0 == h1)
+    (ensures fun h0 r h1 -> h0 == h1 /\ ((r == 0l) ==> (is_poly_pmq h1 z)))
 
 let test_z z =
     let h0 = ST.get () in
     let _ , res = interruptible_for 0ul params_n
-    (fun h _ _ -> live h z /\ h0 == h)
+    (fun h i b -> live h z /\ h0 == h /\ i <= v params_n /\ (~b ==> is_poly_pmq_i h z i))
     (fun i ->
         let zi = z.(i) in
         zi <^ to_elem (-1) *^ (params_B -^ params_U) || zi >^ (params_B -^ params_U)
@@ -1991,6 +1991,16 @@ private let lemma_subpoly_of_pk_is_pk (h: HS.mem) (pk: poly_k) (p: poly) (k: siz
     assert(forall (i:nat{i < v params_n}) . is_pk (bget h p i))
 //#pop-options
 
+#push-options "--print_z3_statistics"
+let lemma_remap_subbuf_indices (w: poly_k) (k: size_t{v k < v params_k}) (h: HS.mem) : Lemma
+    (ensures forall (i:nat{i >= v k * v params_n /\ i < v k * v params_n + v params_n}) . bget h w i == bget h (get_poly w k) (i - v k * v params_n)) =
+    assert(get_poly w k == gsub w (k *! params_n) params_n);
+    assert(forall (i:nat{i >= v k * v params_n /\ i < v k * v params_n + v params_n}) . bget h w i == bget h (get_poly w k) (i - v k * v params_n))
+#pop-options
+
+
+
+
 private inline_for_extraction noextract
 val qtesla_verify_decode_pk_compute_w:
     pk: lbuffer uint8 crypto_publickeybytes
@@ -1999,7 +2009,8 @@ val qtesla_verify_decode_pk_compute_w:
   -> w: poly_k
   -> Stack unit
     (requires fun h -> let bufs = [bb pk; bb c; bb z; bb w] in
-                    BigOps.big_and (live_buf h) bufs /\ BigOps.pairwise_and disjoint_buf bufs)
+                    BigOps.big_and (live_buf h) bufs /\ BigOps.pairwise_and disjoint_buf bufs /\
+                    is_poly_pmq h z)
     (ensures fun h0 _ h1 -> modifies1 w h0 h1 /\ is_poly_k_montgomery h1 w)
 
 //  --log_queries --query_stats --print_z3_statistics 
@@ -2007,6 +2018,7 @@ val qtesla_verify_decode_pk_compute_w:
                 --using_facts_from '* -LowStar.Monotonic.Buffer.unused_in_not_unused_in_disjoint_2'"
 
 let qtesla_verify_decode_pk_compute_w pk c z w =
+    let hInit = ST.get () in
     push_frame();
     let seed = create crypto_seedbytes (u8 0) in
     let pos_list = create params_h 0ul in
@@ -2042,14 +2054,15 @@ let qtesla_verify_decode_pk_compute_w pk c z w =
     assert(is_poly_k_montgomery hAfterPolyUniform a);
     encode_c pos_list sign_list c;
     let hAfterEncodeC = ST.get () in
-    assume(is_poly_pmq hAfterEncodeC z);
+    assert(is_poly_equal hInit hAfterEncodeC z);
     poly_ntt z_ntt z; 
 
     let h1 = ST.get () in
     // All buffers in this stack frame.
     assert(modifies (loc pk_t |+| loc seed |+| loc a |+| loc pos_list |+| loc sign_list |+| loc z_ntt) h0 h1);
-    assert(forall (i:nat{i < v params_n * v params_k}) . bget hAfterDecode pk_t i == bget h1 pk_t i);
-    assert(is_poly_k_pk h1 pk_t);
+    assert(is_poly_k_equal hAfterDecode h1 pk_t);
+    //assert(forall (i:nat{i < v params_n * v params_k}) . bget hAfterDecode pk_t i == bget h1 pk_t i);
+    //assert(is_poly_k_pk h1 pk_t);
     assert(is_poly_k_equal hAfterPolyUniform h1 a);
 
     for 0ul params_k
@@ -2062,7 +2075,7 @@ let qtesla_verify_decode_pk_compute_w pk c z w =
         lemma_sub_poly_is_montgomery hBegin a (get_poly a k) k;
         poly_mul (index_poly w k) (index_poly a k) z_ntt;
         let hAfterMul = ST.get () in
-        assume(is_poly_montgomery hAfterMul (get_poly w k));
+        assert(is_poly_montgomery hAfterMul (get_poly w k));
         let tc_k = index_poly tc k in
         let pk_t_k = sub pk_t (k *! params_n) params_n in
         assert(disjoint tc pk_t);
@@ -2088,11 +2101,16 @@ let qtesla_verify_decode_pk_compute_w pk c z w =
         // Pattern on this line to help establish the line after?
         assert(get_poly w k == gsub w (k *! params_n) params_n);
         assert(forall (i:nat{i < v params_n}) . is_montgomery (bget hEnd (gsub w (k *! params_n) params_n) i));
-        assert(forall (i:nat{i >= v k * v params_n /\ i < v k * v params_n + v params_n}) . {:pattern bget hEnd w i} bget hEnd w i == bget hEnd (gsub w (k *! params_n) params_n) (i - (v k * v params_n)));
-        assert(forall (i:nat{i >= v k * v params_n /\ i < v k * v params_n + v params_n}) . is_montgomery (bget hEnd w i)); 
+        //assert(bget hEnd w (v k * v params_n) == bget hEnd (get_poly w k) 0);
+        assert(get_poly w k == gsub w (k *! params_n) params_n);
+        // For some reason, this fact doesn't prove in this context, but works as its own lemma.
+        lemma_remap_subbuf_indices w k hEnd;
+        assert(forall (i:nat{i >= v k * v params_n /\ i < v k * v params_n + v params_n}) . bget hEnd w i == bget hEnd (get_poly w k) (i - v k * v params_n));
+        //assert(forall (i:nat{i >= v k * v params_n /\ i < v k * v params_n + v params_n}) . is_montgomery (bget hEnd w i)); 
         let pTest = get_poly w k in
         assert(is_montgomery (bget hEnd pTest 0));
         assert(forall (i:nat{i < v k * v params_n}) . is_montgomery (bget hEnd w i));
+        assert(forall (i:nat{i < v params_n}) . is_montgomery (bget hEnd (get_poly w k) i));
         assert(forall (i:nat{i >= v k * v params_n /\ i < v k * v params_n + v params_n}) . is_montgomery (bget hEnd w i));
         assert(is_poly_k_montgomery_i hEnd w (((v k) + 1) * v params_n));
         assert(is_poly_k_equal hBegin hEnd a);
@@ -2120,10 +2138,12 @@ val qtesla_verify_valid_z:
   -> z : poly
   -> Stack bool
     (requires fun h -> let bufs = [bb sm; bb pk; bb c; bb z] in
-                    FStar.BigOps.big_and (live_buf h) bufs /\ FStar.BigOps.pairwise_and disjoint_buf bufs)
+                    FStar.BigOps.big_and (live_buf h) bufs /\ FStar.BigOps.pairwise_and disjoint_buf bufs /\
+                    is_poly_pmq h z)
     (ensures fun h0 _ h1 -> modifies0 h0 h1)
 
 let qtesla_verify_valid_z smlen sm pk c z =
+    let hInit = ST.get () in
     push_frame();
 
     let hm = create crypto_hmbytes (u8 0) in
@@ -2133,6 +2153,7 @@ let qtesla_verify_valid_z smlen sm pk c z =
 
     let h0 = ST.get () in
     assert(modifies0 h0 h0);
+    assert(is_poly_equal hInit h0 z);
     
     qtesla_verify_decode_pk_compute_w pk c z w;
     let h1 = ST.get () in
